vSetDgn: initial pass of trivial cleanups

theories/νSet/νDgnSet.v
@@ -11,31 +11,31 @@ Set Typeclasses Depth 10.
 Remove Printing Let sigT.
 Remove Printing Let prod.
 
-Module νDgnSet (A : νSet.AritySig).
+Module νDgnSet (A: νSet.AritySig).
 Import A.
 
 Module Import νSet := νSet.νSet A.
 
-Definition FramePrev {p k} (deps: DepsRestr p.+1 k) : Type :=
+Definition FramePrev {p k} (deps: DepsRestr p.+1 k): Type :=
   deps.(_frames).2.
 
-Definition FrameBase {p k} (deps: DepsRestr p.+1 k) : Type :=
+Definition FrameBase {p k} (deps: DepsRestr p.+1 k): Type :=
   mkFrame (deps.(1)).
 
-Definition NextDepsRestr {p k} (depsCohs: DepsCohs p k) : DepsRestr p.+1 k :=
+Definition NextDepsRestr {p k} (depsCohs: DepsCohs p k): DepsRestr p.+1 k :=
   mkDepsRestr.
 
-Fixpoint mkReflFrameTypes {p k} : DepsRestr p k -> Type :=
+Fixpoint mkReflFrameTypes {p k}: DepsRestr p k -> Type :=
   match p with
   | 0 => fun _ => unit
   | p'.+1 => fun deps =>
-    { R : mkReflFrameTypes deps.(1) &T
+    { R: mkReflFrameTypes deps.(1) &T
           FramePrev deps -> FrameBase deps }
   end.
 
 Class DepsReflRestr p k := {
-  _deps : DepsRestr p k;
-  _reflFrames : mkReflFrameTypes _deps;
+  _deps: DepsRestr p k;
+  _reflFrames: mkReflFrameTypes _deps;
 }.
 
 #[local]
@@ -53,27 +53,27 @@ Notation "x .(1)" := (proj1DepsRefl x%_depsreflrestr)
   (at level 1, left associativity, format "x .(1)"): depsreflrestr_scope.
 
 
-Definition ReflFramePrev {p k} (deps: DepsReflRestr p.+1 k) : Type :=
+Definition ReflFramePrev {p k} (deps: DepsReflRestr p.+1 k): Type :=
   FramePrev deps.(_deps).
 
-Definition ReflFrameBase {p k} (deps: DepsReflRestr p.+1 k) : Type :=
+Definition ReflFrameBase {p k} (deps: DepsReflRestr p.+1 k): Type :=
   FrameBase deps.(_deps).
 
-Definition restrFrame {p k} i (Hi : i <= k) (deps: DepsRestr p.+1 k) (ε: arity) :
+Definition restrFrame {p k} i (Hi: i <= k) (deps: DepsRestr p.+1 k) (ε: arity):
   FrameBase deps -> FramePrev deps :=
   deps.(_restrFrames).2 i Hi ε.
 
-Definition reflFrame {p k} (deps: DepsReflRestr p.+1 k) :
+Definition reflFrame {p k} (deps: DepsReflRestr p.+1 k):
   ReflFramePrev deps -> ReflFrameBase deps :=
   deps.(_reflFrames).2.
 
 Definition mkIdReflRestrFrameType {p k}
-  (deps: DepsReflRestr p.+1 k) : Type :=
-  forall ε (d : ReflFramePrev deps),
+  (deps: DepsReflRestr p.+1 k): Type :=
+  forall ε (d: ReflFramePrev deps),
   restrFrame k leR_refl deps.(_deps) ε (reflFrame deps d) = d.
 
 Fixpoint mkIdReflRestrFrameTypes {p} :
-  forall {k} (deps : DepsReflRestr p k), Type :=
+  forall {k} (deps: DepsReflRestr p k), Type :=
   match p with
   | 0 => fun _ _ => unit
   | S p =>
@@ -82,29 +82,22 @@ Fixpoint mkIdReflRestrFrameTypes {p} :
       mkIdReflRestrFrameType deps }
   end.
 
-Definition PaintingPrev {p k} (deps: DepsRestr p.+1 k) : FramePrev deps -> Type :=
+Definition PaintingPrev {p k} (deps: DepsRestr p.+1 k):
+  FramePrev deps -> Type :=
   deps.(_paintings).2.
 
 Definition PaintingBase {p k} (deps: DepsRestr p.+1 k) 
-  (extraDeps: DepsRestrExtension p.+1 k deps) : FrameBase deps -> Type :=
+  (extraDeps: DepsRestrExtension p.+1 k deps): FrameBase deps -> Type :=
   (mkPaintings (deps; extraDeps)).2.
 
-Definition ReflPaintingPrev {p k} (deps: DepsReflRestr p.+1 k) :
+Definition ReflPaintingPrev {p k} (deps: DepsReflRestr p.+1 k):
   ReflFramePrev deps -> Type :=
   PaintingPrev deps.(_deps).
 
 Definition ReflPaintingBase {p k} (deps: DepsReflRestr p.+1 k)
-  (extraDeps: DepsRestrExtension p.+1 k deps.(_deps)) :
+  (extraDeps: DepsRestrExtension p.+1 k deps.(_deps)):
   ReflFrameBase deps -> Type :=
   PaintingBase deps.(_deps) extraDeps.
-
-(*
-Definition mkReflPaintingType {p k} {deps: DepsRestr α p.+1 k}
-  `(extraDeps: DepsRestrExtension α p.+1 k deps) :=
-  forall q (Hq: q <= k) ε (d: mkFrame α (proj1DepsRestr α deps)),
-  deps.(_paintings α).2 (deps.(_restrFrames α).2 q _ ε d) ->
-  (mkPaintings α (AddRestrDep α _ deps extraDeps)).2 d.
-*)
 
 Definition mkReflPaintingType {p k} (deps: DepsReflRestr p.+1 k)
   `(extraDeps: DepsRestrExtension p.+1 k deps.(_deps)) :=
@@ -112,8 +105,9 @@ Definition mkReflPaintingType {p k} (deps: DepsReflRestr p.+1 k)
   ReflPaintingPrev deps d ->
   ReflPaintingBase deps extraDeps (reflFrame deps d).
 
-Fixpoint mkReflPaintingTypes {p} :
-  forall {k} (deps : DepsReflRestr p k) `(extraDeps: DepsRestrExtension p k deps.(_deps)), Type :=
+Fixpoint mkReflPaintingTypes {p}:
+  forall {k} (deps: DepsReflRestr p k)
+  `(extraDeps: DepsRestrExtension p k deps.(_deps)), Type :=
   match p with
   | 0 => fun _ _ _ => unit
   | S p =>
@@ -129,114 +123,114 @@ Class CohReflRestrFrameTypeBlock {p k} (deps: DepsRestr p k) := {
 
 #[local]
 Instance toDepsRefl {p k} 
-  (depsCohs : DepsCohs p k)
-  (reflFrames : mkReflFrameTypes depsCohs.(νSet._deps)) : DepsReflRestr p k :=
+  (depsCohs: DepsCohs p k)
+  (reflFrames: mkReflFrameTypes depsCohs.(νSet._deps)): DepsReflRestr p k :=
   {| _deps := depsCohs.(νSet._deps);
      _reflFrames := reflFrames;
   |}.
 
-Definition mkCohReflRestrFrameTypesStep {p k} (deps : DepsCohs p.+1 k)
-  (reflFrames : mkReflFrameTypes deps.(νSet._deps))
+Definition mkCohReflRestrFrameTypesStep {p k} (deps: DepsCohs p.+1 k)
+  (reflFrames: mkReflFrameTypes deps.(νSet._deps))
   (prev: CohReflRestrFrameTypeBlock (NextDepsRestr deps.(1))): Type :=
   { Q: prev.(CohReflRestrFrameTypesDef) &T
-    forall i (Hi: i <= k) (ε : arity) (d : ReflFrameBase (toDepsRefl deps reflFrames)),
-    let reflFrame' : FramePrev _ -> FrameBase _ := (prev.(ReflFramesDef) Q).2 in
+    forall i (Hi: i <= k) (ε: arity) (d: ReflFrameBase (toDepsRefl deps reflFrames)),
+    let reflFrame': FramePrev _ -> FrameBase _ := (prev.(ReflFramesDef) Q).2 in
     reflFrame _ (restrFrame i Hi _ ε d) =
     restrFrame i (↑ Hi) _ ε (reflFrame' d) }.
 
 Definition mkReflLayer {p k} (deps: DepsCohs p.+1 k)
-  (reflFrames : mkReflFrameTypes deps.(νSet._deps))
-  (reflPaintings: mkReflPaintingTypes (toDepsRefl deps reflFrames) deps.(_extraDeps))
+  (reflFrames: mkReflFrameTypes deps.(νSet._deps))
+  (reflPaintings: mkReflPaintingTypes (toDepsRefl deps reflFrames)
+    deps.(_extraDeps))
   (prev: CohReflRestrFrameTypeBlock (NextDepsRestr deps.(1)))
   (cohFrames: mkCohReflRestrFrameTypesStep deps reflFrames prev)
-  (d: ReflFrameBase (toDepsRefl deps reflFrames)) :
+  (d: ReflFrameBase (toDepsRefl deps reflFrames)):
   mkLayer deps.(νSet._deps).(_restrFrames) d ->
   mkLayer
     (NextDepsRestr deps.(1)).(_restrFrames)
     ((prev.(ReflFramesDef) cohFrames.1).2 d) :=
   fun l ε =>
     rew [(NextDepsRestr deps.(1)).(_paintings).2] cohFrames.2 0 leR_O ε d in
-    reflPaintings.2 (restrFrame 0 leR_O (toDepsRefl deps reflFrames).(_deps) ε d) (l ε).
+    reflPaintings.2 (restrFrame 0 leR_O (toDepsRefl deps reflFrames).(_deps)
+      ε d) (l ε).
 
 Fixpoint mkCohReflRestrFrameTypesAndReflFrames {p k}:
   forall
     (deps: DepsCohs p k)
-    (reflFrames : mkReflFrameTypes deps.(νSet._deps))
-    (reflPaintings : mkReflPaintingTypes (toDepsRefl deps reflFrames) deps.(_extraDeps)),
+    (reflFrames: mkReflFrameTypes deps.(νSet._deps))
+    (reflPaintings: mkReflPaintingTypes (toDepsRefl deps reflFrames)
+      deps.(_extraDeps)),
     CohReflRestrFrameTypeBlock (NextDepsRestr deps) :=
   match p with
   | 0 =>
     fun deps reflFrames reflPaintings =>
     {|
       CohReflRestrFrameTypesDef := unit;
-      ReflFramesDef _ := (tt; fun _ => tt) : mkReflFrameTypes (NextDepsRestr deps)
+      ReflFramesDef _ := (tt; fun _ => tt):
+        mkReflFrameTypes (NextDepsRestr deps)
     |}
   | S p =>
     fun deps reflFrames reflPaintings =>
-    let prev := mkCohReflRestrFrameTypesAndReflFrames deps.(1) reflFrames.1 reflPaintings.1 in
+    let prev := mkCohReflRestrFrameTypesAndReflFrames deps.(1)
+      reflFrames.1 reflPaintings.1 in
     {|
-      CohReflRestrFrameTypesDef := mkCohReflRestrFrameTypesStep deps reflFrames prev;
+      CohReflRestrFrameTypesDef := mkCohReflRestrFrameTypesStep deps
+        reflFrames prev;
       ReflFramesDef Q :=
         let prevFrames := prev.(ReflFramesDef) Q.1 in
         let reflFrame d := (prevFrames.2 d.1;
           mkReflLayer deps reflFrames reflPaintings prev Q d.1 d.2) in
-        (prevFrames; reflFrame) : mkReflFrameTypes (NextDepsRestr deps)
+        (prevFrames; reflFrame): mkReflFrameTypes (NextDepsRestr deps)
     |}
   end.
 
 Definition mkCohReflRestrFrameTypes {p k}
   (deps: DepsCohs p k)
   (reflFrames: mkReflFrameTypes deps.(νSet._deps))
-  (reflPaintings: mkReflPaintingTypes (toDepsRefl deps reflFrames) deps.(_extraDeps)) : Type :=
-  (mkCohReflRestrFrameTypesAndReflFrames deps reflFrames reflPaintings).(CohReflRestrFrameTypesDef).
-
-(*
-Definition restrPainting {p k} (deps : DepsReflCohs p.+1 k) : 
-  forall i (Hi: i <= k) (ε : arity) (d : ReflFrameBase (reflOfCohs deps)),
-  ReflPaintingBase (reflOfCohs deps) (extraOfCohs deps) d ->
-  ReflPaintingPrev (reflOfCohs deps) (restrFrame i Hi (restrOfCohs deps) ε d) :=
-  deps.(_depsCohs).(_restrPaintings).2.
-
-Definition reflPainting {p k} (deps : DepsReflCohs p.+1 k) : 
-  forall (d : ReflFramePrev (reflOfCohs deps)),
-  ReflPaintingPrev (reflOfCohs deps) d ->
-  ReflPaintingBase (reflOfCohs deps) (extraOfCohs deps) (reflFrame (reflOfCohs deps) d) :=
-  deps.(_reflPaintingDeps).2.
-*)
+  (reflPaintings: mkReflPaintingTypes (toDepsRefl deps reflFrames)
+    deps.(_extraDeps)): Type :=
+  (mkCohReflRestrFrameTypesAndReflFrames deps reflFrames
+    reflPaintings).(CohReflRestrFrameTypesDef).
 
 Definition mkIdReflRestrPaintingType {p k}
-  (deps : DepsCohs p.+1 k)
-  (reflFrames : mkReflFrameTypes deps.(νSet._deps))
-  (reflPaintings : mkReflPaintingTypes (toDepsRefl deps reflFrames) deps.(_extraDeps))
-  (idReflRestrFrames : mkIdReflRestrFrameTypes (toDepsRefl deps reflFrames)): Type :=
+  (deps: DepsCohs p.+1 k)
+  (reflFrames: mkReflFrameTypes deps.(νSet._deps))
+  (reflPaintings: mkReflPaintingTypes (toDepsRefl deps reflFrames)
+    deps.(_extraDeps))
+  (idReflRestrFrames: mkIdReflRestrFrameTypes (toDepsRefl deps reflFrames)): Type :=
   forall
-    (ε : arity)
-    (d : ReflFramePrev (toDepsRefl deps reflFrames))
-    (c : ReflPaintingPrev (toDepsRefl deps reflFrames) d),
+    (ε: arity)
+    (d: ReflFramePrev (toDepsRefl deps reflFrames))
+    (c: ReflPaintingPrev (toDepsRefl deps reflFrames) d),
   rew [ReflPaintingPrev (toDepsRefl deps reflFrames)] idReflRestrFrames.2 ε d in
   deps.(_restrPaintings).2 k leR_refl ε (reflFrames.2 d) (reflPaintings.2 d c) = c.
 
 Fixpoint mkIdReflRestrPaintingTypes {p} :
   forall {k}
-    (deps : DepsCohs p k)
-    (reflFrames : mkReflFrameTypes deps.(νSet._deps))
-    (reflPaintings : mkReflPaintingTypes (toDepsRefl deps reflFrames) deps.(_extraDeps))
-    (idReflRestrFrames : mkIdReflRestrFrameTypes (toDepsRefl deps reflFrames)), Type :=
+    (deps: DepsCohs p k)
+    (reflFrames: mkReflFrameTypes deps.(νSet._deps))
+    (reflPaintings: mkReflPaintingTypes (toDepsRefl deps reflFrames)
+      deps.(_extraDeps))
+    (idReflRestrFrames: mkIdReflRestrFrameTypes (toDepsRefl deps reflFrames)), 
+    Type :=
   match p with
   | 0 => fun _ _ _ _ _ => unit
   | S p =>
     fun k deps reflFrames reflPaintings idReflRestrFrames =>
     { _: mkIdReflRestrPaintingTypes deps.(1) reflFrames.1 reflPaintings.1 idReflRestrFrames.1 &T
-      mkIdReflRestrPaintingType deps reflFrames reflPaintings idReflRestrFrames }
+      mkIdReflRestrPaintingType deps reflFrames reflPaintings
+        idReflRestrFrames }
   end.
 
 Class DepsReflCohs p k := {
-  _depsCohs2 : DepsCohs2 p k;
-  _reflFrameDeps : mkReflFrameTypes _depsCohs.(νSet._deps);
-  _reflPaintingDeps : mkReflPaintingTypes (toDepsRefl _depsCohs _reflFrameDeps) _depsCohs.(_extraDeps);
-  _idReflRestrFrames : mkIdReflRestrFrameTypes (toDepsRefl _depsCohs _reflFrameDeps);
-  _idReflRestrPaintings : mkIdReflRestrPaintingTypes _depsCohs _reflFrameDeps _reflPaintingDeps _idReflRestrFrames;
-  _cohReflRestrFrames : mkCohReflRestrFrameTypes _depsCohs _reflFrameDeps _reflPaintingDeps
+  _depsCohs2: DepsCohs2 p k;
+  _reflFrameDeps: mkReflFrameTypes _depsCohs.(νSet._deps);
+  _reflPaintingDeps: mkReflPaintingTypes
+    (toDepsRefl _depsCohs _reflFrameDeps) _depsCohs.(_extraDeps);
+  _idReflRestrFrames: mkIdReflRestrFrameTypes
+    (toDepsRefl _depsCohs _reflFrameDeps);
+  _idReflRestrPaintings: mkIdReflRestrPaintingTypes _depsCohs _reflFrameDeps _reflPaintingDeps _idReflRestrFrames;
+  _cohReflRestrFrames: mkCohReflRestrFrameTypes _depsCohs _reflFrameDeps _reflPaintingDeps
 }.
 
 #[local]
@@ -257,66 +251,73 @@ Notation "x .(1)" := (proj1DepsReflCohs x%_depsreflcohs)
   (at level 1, left associativity, format "x .(1)"): depsreflcohs_scope.
 
 Definition ReflOfReflCohs {p k}
-  `(depsCohs: DepsReflCohs p k) : DepsReflRestr p k :=
+  `(depsCohs: DepsReflCohs p k): DepsReflRestr p k :=
 {|
   _deps := depsCohs.(_depsCohs2).(_depsCohs).(νSet._deps);
   _reflFrames := depsCohs.(_reflFrameDeps);
 |}.
 
 Definition RestrOfReflCohs {p k}
-  `(depsCohs: DepsReflCohs p k) : DepsRestr p k :=
+  `(depsCohs: DepsReflCohs p k): DepsRestr p k :=
   (ReflOfReflCohs depsCohs).(_deps).
 
 Definition CohsOfReflCohs {p k}
-  `(depsCohs: DepsReflCohs p k) : DepsCohs p k :=
+  `(depsCohs: DepsReflCohs p k): DepsCohs p k :=
   depsCohs.(_depsCohs2).(_depsCohs).
 
 Definition RestrExtOfReflCohs {p k}
-  `(depsCohs: DepsReflCohs p k) : DepsRestrExtension p k (RestrOfReflCohs depsCohs) :=
+  `(depsCohs: DepsReflCohs p k): DepsRestrExtension p k
+    (RestrOfReflCohs depsCohs) :=
   depsCohs.(_depsCohs2).(_depsCohs).(_extraDeps).
 
 Definition CohsExtOfReflCohs {p k}
-  `(depsCohs: DepsReflCohs p k) : DepsCohsExtension p k (CohsOfReflCohs depsCohs) :=
+  `(depsCohs: DepsReflCohs p k): DepsCohsExtension p k
+    (CohsOfReflCohs depsCohs) :=
   depsCohs.(_depsCohs2).(_extraDepsCohs).
 
-Definition mkReflFrames {p k} (deps : DepsReflCohs p k):
+Definition mkReflFrames {p k} (deps: DepsReflCohs p k):
   mkReflFrameTypes (NextDepsRestr (CohsOfReflCohs deps)) :=
   (mkCohReflRestrFrameTypesAndReflFrames
     deps.(_depsCohs2).(_depsCohs)
     deps.(_reflFrameDeps)
     deps.(_reflPaintingDeps)).(ReflFramesDef) deps.(_cohReflRestrFrames).
 
-Definition mkReflFrame {p k} (deps : DepsReflCohs p.+1 k):
-  FramePrev (NextDepsRestr (CohsOfReflCohs deps)) -> FrameBase (NextDepsRestr (CohsOfReflCohs deps)) :=
+Definition mkReflFrame {p k} (deps: DepsReflCohs p.+1 k):
+  FramePrev (NextDepsRestr (CohsOfReflCohs deps)) ->
+  FrameBase (NextDepsRestr (CohsOfReflCohs deps)) :=
   (mkReflFrames deps).2.
 
-Definition NextDepsRefl {p k} (deps : DepsReflCohs p k) : DepsReflRestr p.+1 k :=
+Definition NextDepsRefl {p k} (deps: DepsReflCohs p k): DepsReflRestr p.+1 k :=
   {| _deps := NextDepsRestr (CohsOfReflCohs deps);
      _reflFrames := mkReflFrames deps
   |}.
 
-Definition restrPainting {p k} (deps : DepsReflCohs p.+1 k) :
-  forall i (Hi: i <= k) (ε : arity) (d : ReflFrameBase (ReflOfReflCohs deps)),
+Definition restrPainting {p k} (deps: DepsReflCohs p.+1 k):
+  forall i (Hi: i <= k) (ε: arity) (d: ReflFrameBase (ReflOfReflCohs deps)),
   ReflPaintingBase (ReflOfReflCohs deps) (RestrExtOfReflCohs deps) d ->
-  ReflPaintingPrev (ReflOfReflCohs deps) (restrFrame i Hi (RestrOfReflCohs deps) ε d) :=
+  ReflPaintingPrev (ReflOfReflCohs deps)
+    (restrFrame i Hi (RestrOfReflCohs deps) ε d) :=
   deps.(_depsCohs2).(_depsCohs).(_restrPaintings).2.
 
-Definition reflPainting {p k} (deps : DepsReflCohs p.+1 k) :
-  forall (d : ReflFramePrev (ReflOfReflCohs deps)),
+Definition reflPainting {p k} (deps: DepsReflCohs p.+1 k):
+  forall (d: ReflFramePrev (ReflOfReflCohs deps)),
   ReflPaintingPrev (ReflOfReflCohs deps) d ->
-  ReflPaintingBase (ReflOfReflCohs deps) (RestrExtOfReflCohs deps) (reflFrame (ReflOfReflCohs deps) d) :=
+  ReflPaintingBase (ReflOfReflCohs deps) (RestrExtOfReflCohs deps)
+    (reflFrame (ReflOfReflCohs deps) d) :=
   deps.(_reflPaintingDeps).2.
 
 Definition mkIdReflRestrLayer {p k}
-  (deps : DepsReflCohs p.+1 k)
-  (ε : arity)
-  (d : ReflFrameBase (ReflOfReflCohs deps))
-  (l : mkLayer (RestrOfReflCohs deps).(_restrFrames) d) 
-  (prevIdReflRestrFrames : mkIdReflRestrFrameTypes (NextDepsRefl deps.(1))):
+  (deps: DepsReflCohs p.+1 k)
+  (ε: arity)
+  (d: ReflFrameBase (ReflOfReflCohs deps))
+  (l: mkLayer (RestrOfReflCohs deps).(_restrFrames) d) 
+  (prevIdReflRestrFrames: mkIdReflRestrFrameTypes (NextDepsRefl deps.(1))):
   rew [mkLayer _] prevIdReflRestrFrames.2 ε d in
-  mkRestrLayer deps.(_depsCohs2).(_depsCohs).(_restrPaintings) (deps.(_depsCohs2).(_depsCohs).(_cohs)) k leR_refl ε _
-    (mkReflLayer deps.(_depsCohs2).(_depsCohs) ((ReflOfReflCohs deps).(_reflFrames)) deps.(_reflPaintingDeps) _
-      deps.(_cohReflRestrFrames) d l) = l.
+  mkRestrLayer deps.(_depsCohs2).(_depsCohs).(_restrPaintings)
+    (deps.(_depsCohs2).(_depsCohs).(_cohs)) k leR_refl ε _
+      (mkReflLayer deps.(_depsCohs2).(_depsCohs)
+        ((ReflOfReflCohs deps).(_reflFrames)) deps.(_reflPaintingDeps) _
+          deps.(_cohReflRestrFrames) d l) = l.
 Proof.
   apply functional_extensionality_dep.
   intros θ.
@@ -330,45 +331,42 @@ Proof.
     (f := fun x => (deps.(_depsCohs2).(_depsCohs).(νSet._deps).(_restrFrames).2 0 leR_O θ x)).
   rewrite rew_map with
     (P := fun x => deps.(_depsCohs2).(_depsCohs).(νSet._deps).(_paintings).2 x)
-    (f := fun x => ((deps.(_depsCohs2).(_depsCohs).(νSet._deps).(_restrFrames).2 k leR_refl ε x))).
+    (f := fun x => ((deps.(_depsCohs2).(_depsCohs).(νSet._deps).(
+      _restrFrames).2 k leR_refl ε x))).
   rewrite 2 rew_compose.
-  apply rew_swap with (P := fun x => deps.(_depsCohs2).(_depsCohs).(νSet._deps).(_paintings).2 x).
-  rewrite rew_app_rl.
-  - reflexivity.
-  - apply (RestrOfReflCohs deps).(_frames).2.(UIP).
+  apply rew_swap with (P := fun x =>
+    deps.(_depsCohs2).(_depsCohs).(νSet._deps).(_paintings).2 x).
+  rewrite rew_app_rl. now trivial.
+  now apply (RestrOfReflCohs deps).(_frames).2.(UIP).
 Defined.
 
-Fixpoint mkIdReflRestrFrames {p k} (deps : DepsReflCohs p k):
+Fixpoint mkIdReflRestrFrames {p k} (deps: DepsReflCohs p k):
   mkIdReflRestrFrameTypes (NextDepsRefl deps).
   destruct p.
-  - simpl.
-    unshelve econstructor.
-    + exact tt.
-    + intros ε [].
-      reflexivity.
+  - simpl. unshelve econstructor. now exact tt. now intros ε [].
   - set (h := mkIdReflRestrFrames p k.+1 deps.(1)%depsreflcohs).
     unshelve econstructor.
-    + apply h.
+    + now apply h.
     + intros ε [l c].
       unshelve eapply eq_existT_curried.
-      * exact (h.2 ε l).
-      * exact (mkIdReflRestrLayer deps ε l c h).
+      * now exact (h.2 ε l).
+      * now exact (mkIdReflRestrLayer deps ε l c h).
 Defined.
 
-Definition mkIdReflRestrFrame {p k} (deps : DepsReflCohs p k):
+Definition mkIdReflRestrFrame {p k} (deps: DepsReflCohs p k):
   mkIdReflRestrFrameType (NextDepsRefl deps) :=
   (mkIdReflRestrFrames deps).2.
 
-Definition HasRefl {p} (deps : DepsReflCohs p 0)
-  (E: mkFrame (NextDepsRestr (CohsOfReflCohs deps)) -> HSet) : Type :=
-  forall (d : FramePrev (NextDepsRestr (CohsOfReflCohs deps)))
-         (c : PaintingPrev (NextDepsRestr (CohsOfReflCohs deps)) d),
+Definition HasRefl {p} (deps: DepsReflCohs p 0)
+  (E: mkFrame (NextDepsRestr (CohsOfReflCohs deps)) -> HSet): Type :=
+  forall (d: FramePrev (NextDepsRestr (CohsOfReflCohs deps)))
+         (c: PaintingPrev (NextDepsRestr (CohsOfReflCohs deps)) d),
   let l ε := (rew <- mkIdReflRestrFrame deps ε d in c) in
   E (reflFrame (NextDepsRefl deps) d; l).
 
 Inductive DepsReflCohsExtension p: forall k (deps: DepsReflCohs p k), Type :=
 | TopReflCohDep `{deps: DepsReflCohs p 0}
-  (L : HasRefl deps (mkPaintings (mkExtraDeps (CohsExtOfReflCohs deps))).2) :
+  (L: HasRefl deps (mkPaintings (mkExtraDeps (CohsExtOfReflCohs deps))).2):
   DepsReflCohsExtension p 0 deps
 | AddReflCohDep {k} (deps: DepsReflCohs p.+1 k):
   DepsReflCohsExtension p.+1 k deps -> DepsReflCohsExtension p k.+1 deps.(1).
@@ -384,31 +382,31 @@ Notation "( x ; y )" := (AddReflCohDep x y)
 
 
 Fixpoint mkReflPainting {p k}
-  (deps : DepsReflCohs p k)
-  (extraDeps : DepsReflCohsExtension p k deps):
+  (deps: DepsReflCohs p k)
+  (extraDeps: DepsReflCohsExtension p k deps):
   mkReflPaintingType (NextDepsRefl deps) (mkExtraDeps (CohsExtOfReflCohs deps)).
 Proof.
   intros d c.
   destruct extraDeps.
   - unshelve econstructor.
-    + intros ε.
-      exact (rew <- mkIdReflRestrFrame deps ε d in c).
-    + exact (L d c).
+    + intros ε. now exact (rew <- mkIdReflRestrFrame deps ε d in c).
+    + now exact (L d c).
   - destruct c as [l c'].
     unshelve econstructor.
     + apply mkReflLayer.
-      * exact (deps.(_reflPaintingDeps)).
-      * exact l.
-    + exact (mkReflPainting p.+1 k deps extraDeps (d; l) c').
+      * now exact (deps.(_reflPaintingDeps)).
+      * now exact l.
+    + now exact (mkReflPainting p.+1 k deps extraDeps (d; l) c').
 Defined.
 
 Fixpoint mkReflPaintingsPrefix {p k}:
   forall
-    (deps : DepsReflCohs p k)
-    (extraDeps : DepsReflCohsExtension p k deps),
+    (deps: DepsReflCohs p k)
+    (extraDeps: DepsReflCohsExtension p k deps),
   mkReflPaintingTypes
     ((NextDepsRefl deps).(1))
-    (NextDepsRestr (CohsOfReflCohs deps); mkExtraDeps (CohsExtOfReflCohs deps)) :=
+    (NextDepsRestr (CohsOfReflCohs deps);
+    mkExtraDeps (CohsExtOfReflCohs deps)) :=
   match p with
   | 0 => fun _ _ => tt
   | S p =>
@@ -419,19 +417,19 @@ Fixpoint mkReflPaintingsPrefix {p k}:
 
 Definition mkReflPaintings {p k}:
   forall
-    (deps : DepsReflCohs p k)
+    (deps: DepsReflCohs p k)
     (extraDeps: DepsReflCohsExtension p k deps),
-  mkReflPaintingTypes (NextDepsRefl deps) (mkExtraDeps (CohsExtOfReflCohs deps)) :=
+  mkReflPaintingTypes (NextDepsRefl deps)
+    (mkExtraDeps (CohsExtOfReflCohs deps)) :=
   fun deps extraDeps =>
     (mkReflPaintingsPrefix deps extraDeps; mkReflPainting deps extraDeps).
 
 Definition mkCohReflRestrPaintingType {p k}
-  (deps : DepsReflCohs p.+1 k)
-  (extraDeps : DepsReflCohsExtension p.+1 k deps) : Type :=
-  forall
-    (ε : arity) i (Hi: i <= k)
-    (d : ReflFrameBase (ReflOfReflCohs deps))
-    (c : ReflPaintingBase (ReflOfReflCohs deps) (RestrExtOfReflCohs deps) d),
+  (deps: DepsReflCohs p.+1 k)
+  (extraDeps: DepsReflCohsExtension p.+1 k deps): Type :=
+  forall (ε: arity) i (Hi: i <= k)
+    (d: ReflFrameBase (ReflOfReflCohs deps))
+    (c: ReflPaintingBase (ReflOfReflCohs deps) (RestrExtOfReflCohs deps) d),
   rew [ReflPaintingBase
         (toDepsRefl deps.(_depsCohs2).(_depsCohs) deps.(_reflFrameDeps))
         deps.(_depsCohs2).(_depsCohs).(_extraDeps)]
@@ -442,9 +440,8 @@ Definition mkCohReflRestrPaintingType {p k}
     (mkReflPainting deps.(1) (deps; extraDeps) d c).
 
 Fixpoint mkCohReflRestrPaintingTypes {p} :
-  forall {k}
-    (deps : DepsReflCohs p k)
-    (extraDeps : DepsReflCohsExtension p k deps), Type :=
+  forall {k} (deps: DepsReflCohs p k)
+    (extraDeps: DepsReflCohsExtension p k deps), Type :=
   match p with
   | 0 => fun _ _ _ => unit
   | S p =>
@@ -454,8 +451,8 @@ Fixpoint mkCohReflRestrPaintingTypes {p} :
   end. 
 
 Fixpoint mkIdReflRestrPainting {p k}
-  (deps : DepsReflCohs p k)
-  (extraDeps : DepsReflCohsExtension p k deps):
+  (deps: DepsReflCohs p k)
+  (extraDeps: DepsReflCohsExtension p k deps):
   mkIdReflRestrPaintingType
     (mkDepsCohs deps.(_depsCohs2))
     (mkReflFrames deps)
@@ -467,23 +464,21 @@ Proof.
   - destruct deps, _depsCohs3.
     generalize dependent _extraDepsCohs0; intro.
     refine (match _extraDepsCohs0 with TopCohDep E => _ end).
-    intros.
-    simpl.
+    intros; simpl.
     rewrite rew_compose.
     set (e := (mkIdReflRestrFrames _).2 ε d0).
-    enough (eq_sym e • e = eq_refl) as ->.
-    * reflexivity.
-    * apply (mkFrame _).(UIP).
+    enough (eq_sym e • e = eq_refl) as ->. now trivial.
+    now apply (mkFrame _).(UIP).
   - unshelve eapply (eq_existT_curried_dep  
       (Q := mkPainting deps .(_depsCohs2) .(_depsCohs) .(_extraDeps))).
-    * apply mkIdReflRestrLayer.
+    * now apply mkIdReflRestrLayer.
     * destruct c as [l c].
-      exact (mkIdReflRestrPainting p.+1 k deps extraDeps ε (d; l) c).
+      now exact (mkIdReflRestrPainting p.+1 k deps extraDeps ε (d; l) c).
 Defined.
 
 Fixpoint mkIdReflRestrPaintings {p k}
-  (deps : DepsReflCohs p k)
-  (extraDeps : DepsReflCohsExtension p k deps):
+  (deps: DepsReflCohs p k)
+  (extraDeps: DepsReflCohsExtension p k deps):
   mkIdReflRestrPaintingTypes
     (mkDepsCohs deps.(_depsCohs2))
     (mkReflFrames deps)
@@ -491,50 +486,52 @@ Fixpoint mkIdReflRestrPaintings {p k}
     (mkIdReflRestrFrames deps).
 Proof.
   destruct p.
+  - unshelve econstructor. now exact tt. now apply mkIdReflRestrPainting.
   - unshelve econstructor.
-    + exact tt.
-    + apply mkIdReflRestrPainting.
-  - unshelve econstructor.
-    + exact (mkIdReflRestrPaintings p k.+1 deps.(1)%depsreflcohs (deps; extraDeps)%extradepsreflcohs).
-    + apply mkIdReflRestrPainting.
+    + now exact (mkIdReflRestrPaintings p k.+1 deps.(1)%depsreflcohs
+      (deps; extraDeps)%extradepsreflcohs).
+    + now apply mkIdReflRestrPainting.
 Defined.
 
 Class DepsReflCohs2 p k := {
   _depsReflCohs: DepsReflCohs p k;
-  _extraDepsCohs2 : DepsCohs2Extension p k _depsReflCohs.(_depsCohs2);
+  _extraDepsCohs2: DepsCohs2Extension p k _depsReflCohs.(_depsCohs2);
   _extraDepsRefl: DepsReflCohsExtension p k _depsReflCohs;
   _cohReflRestrPaintings: mkCohReflRestrPaintingTypes _depsReflCohs _extraDepsRefl;
 }.
 
 Definition Cohs2OfReflCohs2 {p k}
-  (depsCohs2: DepsReflCohs2 p k) : DepsCohs2 p k :=
+  (depsCohs2: DepsReflCohs2 p k): DepsCohs2 p k :=
   depsCohs2.(_depsReflCohs).(_depsCohs2).
 
 Definition ReflOfReflCohs2 {p k}
-  `(depsCohs2: DepsReflCohs2 p k) : DepsReflRestr p k :=
+  `(depsCohs2: DepsReflCohs2 p k): DepsReflRestr p k :=
   ReflOfReflCohs (depsCohs2.(_depsReflCohs)).
 
 Definition RestrOfReflCohs2 {p k}
-  `(depsCohs2: DepsReflCohs2 p k) : DepsRestr p k :=
+  `(depsCohs2: DepsReflCohs2 p k): DepsRestr p k :=
   (ReflOfReflCohs (depsCohs2.(_depsReflCohs))).(_deps).
 
 Definition CohsOfReflCohs2 {p k}
-  `(depsCohs2: DepsReflCohs2 p k) : DepsCohs p k :=
+  `(depsCohs2: DepsReflCohs2 p k): DepsCohs p k :=
   depsCohs2.(_depsReflCohs).(_depsCohs2).(_depsCohs).
 
 Definition RestrExtOfReflCohs2 {p k}
-  `(depsCohs2: DepsReflCohs2 p k) : DepsRestrExtension p k (RestrOfReflCohs2 depsCohs2) :=
+  `(depsCohs2: DepsReflCohs2 p k): DepsRestrExtension p k
+    (RestrOfReflCohs2 depsCohs2) :=
   depsCohs2.(_depsReflCohs).(_depsCohs2).(_depsCohs).(_extraDeps).
 
 Definition CohsExtOfReflCohs2 {p k}
-  `(depsCohs2: DepsReflCohs2 p k) : DepsCohsExtension p k (CohsOfReflCohs2 depsCohs2) :=
+  `(depsCohs2: DepsReflCohs2 p k): DepsCohsExtension p k
+    (CohsOfReflCohs2 depsCohs2) :=
   depsCohs2.(_depsReflCohs).(_depsCohs2).(_extraDepsCohs).
 
 #[local]
 Instance proj1DepsReflCohs2 {p k} (depsCohs2: DepsReflCohs2 p.+1 k): DepsReflCohs2 p k.+1 :=
 {|
   _depsReflCohs := depsCohs2.(_depsReflCohs).(1);
-  _extraDepsCohs2 := (depsCohs2.(_depsReflCohs).(_depsCohs2); depsCohs2.(_extraDepsCohs2));
+  _extraDepsCohs2 := (depsCohs2.(_depsReflCohs).(_depsCohs2);
+    depsCohs2.(_extraDepsCohs2));
   _extraDepsRefl := (depsCohs2.(_depsReflCohs); depsCohs2.(_extraDepsRefl));
   _cohReflRestrPaintings := depsCohs2.(_cohReflRestrPaintings).1;
 |}.
@@ -546,22 +543,23 @@ Notation "x .(1)" := (proj1DepsReflCohs2 x%depsreflcohs2)
   (at level 1, left associativity, format "x .(1)"): depsreflcohs2_scope.
 
 Definition mkCohReflRestrLayer {p k}
-  (deps : DepsReflCohs2 p.+1 k)
-  (ε : arity) i (Hi : i <= k)
-  (d : mkFrame (((toDepsRefl
-        (mkDepsCohs (Cohs2OfReflCohs2 deps))
-        (mkReflFrames deps.(_depsReflCohs)))).(_deps).(1).(1)))
-  (l : mkLayer (toDepsRefl
-        (mkDepsCohs (Cohs2OfReflCohs2 deps))
-        (mkReflFrames deps.(_depsReflCohs))).(_deps).(1).(_restrFrames) d) 
-  (prevCohReflRestrFrames : 
+  (deps: DepsReflCohs2 p.+1 k)
+  (ε: arity) i (Hi: i <= k)
+  (d: mkFrame (((toDepsRefl
+    (mkDepsCohs (Cohs2OfReflCohs2 deps))
+    (mkReflFrames deps.(_depsReflCohs)))).(_deps).(1).(1)))
+  (l: mkLayer (toDepsRefl
+    (mkDepsCohs (Cohs2OfReflCohs2 deps))
+    (mkReflFrames deps.(_depsReflCohs))).(_deps).(1).(_restrFrames) d) 
+  (prevCohReflRestrFrames: 
     mkCohReflRestrFrameTypes (mkDepsCohs (Cohs2OfReflCohs2 deps).(1))
       (mkReflFrames deps.(_depsReflCohs).(1))
       (mkReflPaintings deps.(_depsReflCohs).(1) (deps.(_depsReflCohs); deps.(_extraDepsRefl)))):
   rew [mkLayer _] prevCohReflRestrFrames.2 i.+1 (⇑ Hi) ε d in
   mkReflLayer
       (CohsOfReflCohs2 deps) deps.(_depsReflCohs).(_reflFrameDeps)
-      deps.(_depsReflCohs).(_reflPaintingDeps) _ deps.(_depsReflCohs).(_cohReflRestrFrames) _
+        deps.(_depsReflCohs).(_reflPaintingDeps) _
+        deps.(_depsReflCohs).(_cohReflRestrFrames) _
     (mkRestrLayer
       (CohsOfReflCohs2 deps).(_restrPaintings)
       (CohsOfReflCohs2 deps).(_cohs) i Hi ε d l) =
@@ -569,8 +567,11 @@ Definition mkCohReflRestrLayer {p k}
       (mkDepsCohs (Cohs2OfReflCohs2 deps)).(1).(_restrPaintings)
       (mkDepsCohs (Cohs2OfReflCohs2 deps)).(1).(_cohs) i (↑ Hi) ε _
     (mkReflLayer
-      (mkDepsCohs (Cohs2OfReflCohs2 deps).(1)) (mkReflFrames deps.(_depsReflCohs).(1))
-      (mkReflPaintings deps.(_depsReflCohs).(1) (deps.(_depsReflCohs); deps.(_extraDepsRefl))) _ prevCohReflRestrFrames d l).
+      (mkDepsCohs (Cohs2OfReflCohs2 deps).(1))
+        (mkReflFrames deps.(_depsReflCohs).(1))
+        (mkReflPaintings deps.(_depsReflCohs).(1)
+        (deps.(_depsReflCohs); deps.(_extraDepsRefl))) _
+        prevCohReflRestrFrames d l).
 Proof.
   apply functional_extensionality_dep.
   intros θ.
@@ -578,8 +579,8 @@ Proof.
   rewrite <- map_subst_app, <- !map_subst.
 
   set (d0 := restrFrame 0 leR_O (toDepsRefl
-              (mkDepsCohs (Cohs2OfReflCohs2 deps).(1))
-              (mkReflFrames deps.(_depsReflCohs).(1))).(_deps) θ d).
+    (mkDepsCohs (Cohs2OfReflCohs2 deps).(1))
+    (mkReflFrames deps.(_depsReflCohs).(1))).(_deps) θ d).
 
   assert (h :
     (mkDepsCohs (Cohs2OfReflCohs2 deps)).(1).(_restrPaintings).2 i (↑ Hi) ε
@@ -602,55 +603,55 @@ Proof.
     (P := fun rf => ReflPaintingBase _ _ rf)
     (f := fun d0 => reflFrame (toDepsRefl _ _) d0).
   rewrite rew_map with
-    (P := fun b => (mkDepsCohs (Cohs2OfReflCohs2 deps)).(1).(νSet._deps).(_paintings).2 b)
-    (f := fun d0 => (mkDepsCohs (Cohs2OfReflCohs2 deps)).(1).(νSet._deps).(_restrFrames).2 i (↑ Hi) ε d0).
+    (P := fun b => (mkDepsCohs (Cohs2OfReflCohs2 deps)).(1).(
+        νSet._deps).(_paintings).2 b)
+    (f := fun d0 => (mkDepsCohs (Cohs2OfReflCohs2 deps)).(1).(
+      νSet._deps).(_restrFrames).2 i (↑ Hi) ε d0).
   rewrite 4 rew_compose.
   apply rew_swap with
-    (P := fun b => (mkDepsCohs (Cohs2OfReflCohs2 deps)).(1).(νSet._deps).(_paintings).2 b).
+    (P := fun b => (mkDepsCohs (Cohs2OfReflCohs2 deps)).(1).(
+      νSet._deps).(_paintings).2 b).
   rewrite rew_app_rl.
   - reflexivity.
   - apply (mkFrame (RestrOfReflCohs2 deps).(1)).(UIP).
 Defined.
 
-Fixpoint mkCohReflRestrFrames {p k} (deps : DepsReflCohs2 p k):
+Fixpoint mkCohReflRestrFrames {p k} (deps: DepsReflCohs2 p k):
   mkCohReflRestrFrameTypes
     (mkDepsCohs (Cohs2OfReflCohs2 deps))
     (mkReflFrames deps.(_depsReflCohs))
     (mkReflPaintings deps.(_depsReflCohs) deps.(_extraDepsRefl)).
 Proof.
   destruct p.
-  - unshelve econstructor.
-    + exact tt.
-    + intros i Hi ε [].
-      reflexivity.
+  - unshelve econstructor. now exact tt. now intros i Hi ε [].
   - set (h := mkCohReflRestrFrames p k.+1 deps.(1)%depsreflcohs2).
     unshelve econstructor.
-    + apply h.
+    + now apply h.
     + intros i Hi ε [l c].
       unshelve eapply eq_existT_curried.
-      * exact (h.2 i.+1 (⇑ Hi) ε l).
-      * exact (mkCohReflRestrLayer deps ε i Hi l c h).
+      * now exact (h.2 i.+1 (⇑ Hi) ε l).
+      * now exact (mkCohReflRestrLayer deps ε i Hi l c h).
 Defined.
 
 Instance mkDepsReflCohs {p k} (deps: DepsReflCohs2 p k): DepsReflCohs p.+1 k.
 Proof.
   unshelve econstructor.
   - unshelve econstructor.
-    + exact (mkDepsCohs (Cohs2OfReflCohs2 deps)).
-    + exact (mkExtraCohs deps.(_extraDepsCohs2)).
-    + apply mkCohPaintings.
-  - apply mkReflFrames.
-  - exact (mkReflPaintings _ (deps.(_extraDepsRefl))).
-  - apply mkIdReflRestrFrames.
-  - apply mkIdReflRestrPaintings.
-  - apply mkCohReflRestrFrames.
+    + now exact (mkDepsCohs (Cohs2OfReflCohs2 deps)).
+    + now exact (mkExtraCohs deps.(_extraDepsCohs2)).
+    + now apply mkCohPaintings.
+  - now apply mkReflFrames.
+  - now exact (mkReflPaintings _ (deps.(_extraDepsRefl))).
+  - now apply mkIdReflRestrFrames.
+  - now apply mkIdReflRestrPaintings.
+  - now apply mkCohReflRestrFrames.
 Defined.
 
 Inductive DepsReflCohs2Extension p: forall k (deps: DepsReflCohs2 p k), Type :=
 | TopReflCohDep2 `{deps: DepsReflCohs2 p 0}
-  (L : HasRefl
+  (L: HasRefl
     (mkDepsReflCohs deps)
-    (mkPaintings (mkExtraDeps (CohsExtOfReflCohs (mkDepsReflCohs deps)))).2) :
+    (mkPaintings (mkExtraDeps (CohsExtOfReflCohs (mkDepsReflCohs deps)))).2):
   DepsReflCohs2Extension p 0 deps
 | AddReflCohDep2 {k} (deps: DepsReflCohs2 p.+1 k):
   DepsReflCohs2Extension p.+1 k deps -> DepsReflCohs2Extension p k.+1 deps.(1)%depsreflcohs2.
@@ -675,9 +676,10 @@ Proof.
 Defined.
 
 Fixpoint mkCohReflRestrPainting {p k}
-  (deps : DepsReflCohs2 p k)
-  (extraDeps : DepsReflCohs2Extension p k deps):
-  mkCohReflRestrPaintingType (mkDepsReflCohs deps) (mkExtraReflCohs deps extraDeps).
+  (deps: DepsReflCohs2 p k)
+  (extraDeps: DepsReflCohs2Extension p k deps):
+  mkCohReflRestrPaintingType (mkDepsReflCohs deps)
+    (mkExtraReflCohs deps extraDeps).
 Proof.
   intros ε i Hi d [l c].
   destruct i.
@@ -697,59 +699,59 @@ Proof.
 Defined.
 
 Fixpoint mkCohReflRestrPaintings {p k}
-  (deps : DepsReflCohs2 p k)
-  (extraDeps : DepsReflCohs2Extension p k deps):
-  mkCohReflRestrPaintingTypes (mkDepsReflCohs deps) (mkExtraReflCohs deps extraDeps).
+  (deps: DepsReflCohs2 p k)
+  (extraDeps: DepsReflCohs2Extension p k deps):
+  mkCohReflRestrPaintingTypes (mkDepsReflCohs deps)
+    (mkExtraReflCohs deps extraDeps).
 Proof.
   destruct p.
+  - unshelve econstructor. now exact tt. now apply mkCohReflRestrPainting.
   - unshelve econstructor.
-    + exact tt.
-    + apply mkCohReflRestrPainting.
-  - unshelve econstructor.
-    + exact (mkCohReflRestrPaintings p k.+1 deps.(1)%depsreflcohs2 (deps; extraDeps)%extradepsreflcohs2).
-    + apply mkCohReflRestrPainting.
+    + now exact (mkCohReflRestrPaintings p k.+1 deps.(1)%depsreflcohs2
+      (deps; extraDeps)%extradepsreflcohs2).
+    + now apply mkCohReflRestrPainting.
 Defined.
 
-Definition dgnDepsRestr {p} (C : νSetData p) : DepsRestr p 0 :=
+Definition dgnDepsRestr {p} (C: νSetData p): DepsRestr p 0 :=
   toDepsRestr C.(restrFrames).
 
-Definition dgnDepsRefl {p} (C : νSetData p)
-  (reflFrames : mkReflFrameTypes (dgnDepsRestr C)) : DepsReflRestr p 0 :=
+Definition dgnDepsRefl {p} (C: νSetData p)
+  (reflFrames: mkReflFrameTypes (dgnDepsRestr C)): DepsReflRestr p 0 :=
   {|
     _deps := dgnDepsRestr C;
     _reflFrames := reflFrames;
   |}.
 
-Definition dgnDepsCohs {p} (C : νSetData p)
-  (E : mkFrame (dgnDepsRestr C) -> HSet) : DepsCohs p 0 :=
+Definition dgnDepsCohs {p} (C: νSetData p)
+  (E: mkFrame (dgnDepsRestr C) -> HSet): DepsCohs p 0 :=
   toDepsCohs
     (deps := dgnDepsRestr C)
     (extraDeps := TopRestrDep (deps := dgnDepsRestr C) E)
     (restrPaintings := C.(restrPaintings) E)
     (C.(cohFrames) E).
 
-Definition dgnDepsCohs2 {p} (C : νSetData p)
-  (E : mkFrame (dgnDepsRestr C) -> HSet)
-  (E' : mkFrame (dgnDepsRestr (mkνSetData p C E)) -> HSet) :
+Definition dgnDepsCohs2 {p} (C: νSetData p)
+  (E: mkFrame (dgnDepsRestr C) -> HSet)
+  (E': mkFrame (dgnDepsRestr (mkνSetData p C E)) -> HSet):
   DepsCohs2 p 0 :=
   toDepsCohs2
     (depsCohs := dgnDepsCohs C E)
     (extraDepsCohs := TopCohDep (depsCohs := dgnDepsCohs C E) E')
     (C.(cohPaintings) E E').
 
-Definition dgnDepsReflCohs {p} (C : νSetData p)
-  (E : mkFrame (dgnDepsRestr C) -> HSet)
-  (E' : mkFrame (dgnDepsRestr (mkνSetData p C E)) -> HSet)
-  (reflFrames : mkReflFrameTypes (dgnDepsRestr C))
-  (reflPaintings : mkReflPaintingTypes
+Definition dgnDepsReflCohs {p} (C: νSetData p)
+  (E: mkFrame (dgnDepsRestr C) -> HSet)
+  (E': mkFrame (dgnDepsRestr (mkνSetData p C E)) -> HSet)
+  (reflFrames: mkReflFrameTypes (dgnDepsRestr C))
+  (reflPaintings: mkReflPaintingTypes
     (dgnDepsRefl C reflFrames)
     (TopRestrDep (deps := dgnDepsRestr C) E))
-  (idReflRestrFrames : mkIdReflRestrFrameTypes (dgnDepsRefl C reflFrames))
+  (idReflRestrFrames: mkIdReflRestrFrameTypes (dgnDepsRefl C reflFrames))
   (idReflRestrPaintings :
     mkIdReflRestrPaintingTypes (dgnDepsCohs C E)
       reflFrames reflPaintings idReflRestrFrames)
   (cohRestrReflFrames :
-    mkCohReflRestrFrameTypes (dgnDepsCohs C E) reflFrames reflPaintings) :
+    mkCohReflRestrFrameTypes (dgnDepsCohs C E) reflFrames reflPaintings):
   DepsReflCohs p 0 :=
   {|
     _depsCohs2 := dgnDepsCohs2 C E E';
@@ -760,21 +762,21 @@ Definition dgnDepsReflCohs {p} (C : νSetData p)
     _cohReflRestrFrames := cohRestrReflFrames;
   |}.
 
-Definition dgnHasRefl {p} (C : νSetData p)
-  (E : mkFrame (dgnDepsRestr C) -> HSet)
-  (E' : mkFrame (dgnDepsRestr (mkνSetData p C E)) -> HSet)
-  (reflFrames : mkReflFrameTypes (dgnDepsRestr C))
+Definition dgnHasRefl {p} (C: νSetData p)
+  (E: mkFrame (dgnDepsRestr C) -> HSet)
+  (E': mkFrame (dgnDepsRestr (mkνSetData p C E)) -> HSet)
+  (reflFrames: mkReflFrameTypes (dgnDepsRestr C))
   (reflPaintings :
     mkReflPaintingTypes
       (dgnDepsRefl C reflFrames)
       (TopRestrDep (deps := dgnDepsRestr C) E))
-  (idReflRestrFrames : mkIdReflRestrFrameTypes (dgnDepsRefl C reflFrames))
+  (idReflRestrFrames: mkIdReflRestrFrameTypes (dgnDepsRefl C reflFrames))
   (idReflRestrPaintings :
     mkIdReflRestrPaintingTypes (dgnDepsCohs C E)
       reflFrames reflPaintings idReflRestrFrames)
   (cohRestrReflFrames :
     mkCohReflRestrFrameTypes (dgnDepsCohs C E)
-      reflFrames reflPaintings) : Type :=
+      reflFrames reflPaintings): Type :=
   HasRefl
     (dgnDepsReflCohs C E E'
       reflFrames reflPaintings
@@ -788,72 +790,73 @@ Definition dgnHasRefl {p} (C : νSetData p)
             idReflRestrFrames idReflRestrPaintings
             cohRestrReflFrames)))).2.
 
-Class DgnData {p} (C : νSetData p)
-  (E : mkFrame (dgnDepsRestr C) -> HSet) := {
-  reflFrames : mkReflFrameTypes (dgnDepsRestr C);
+Class DgnData {p} (C: νSetData p)
+  (E: mkFrame (dgnDepsRestr C) -> HSet) := {
+  reflFrames: mkReflFrameTypes (dgnDepsRestr C);
   reflPaintings :
     mkReflPaintingTypes
       (dgnDepsRefl C reflFrames)
       (TopRestrDep (deps := dgnDepsRestr C) E);
-  idReflRestrFrames : mkIdReflRestrFrameTypes (dgnDepsRefl C reflFrames);
+  idReflRestrFrames: mkIdReflRestrFrameTypes (dgnDepsRefl C reflFrames);
   idReflRestrPaintings :
     mkIdReflRestrPaintingTypes
       (dgnDepsCohs C E) reflFrames reflPaintings idReflRestrFrames;
-  cohRestrReflFrames (E' : mkFrame (dgnDepsRestr (mkνSetData p C E)) -> HSet):
+  cohRestrReflFrames (E': mkFrame (dgnDepsRestr (mkνSetData p C E)) -> HSet):
     mkCohReflRestrFrameTypes (dgnDepsCohs C E) reflFrames reflPaintings;
   cohReflRestrPaintings
-    (E' : mkFrame (dgnDepsRestr (mkνSetData p C E)) -> HSet)
-    (L : dgnHasRefl C E E'
-            reflFrames reflPaintings
-            idReflRestrFrames idReflRestrPaintings
-            (cohRestrReflFrames E')) :
+    (E': mkFrame (dgnDepsRestr (mkνSetData p C E)) -> HSet)
+    (L: dgnHasRefl C E E'
+      reflFrames reflPaintings
+      idReflRestrFrames idReflRestrPaintings
+      (cohRestrReflFrames E')):
     mkCohReflRestrPaintingTypes _ (TopReflCohDep L);
 }.
 
 Definition dgnDepsReflCohsFromData {p}
-  (C : νSetData p)
-  (E : mkFrame (dgnDepsRestr C) -> HSet)
-  (E' : mkFrame (dgnDepsRestr (mkνSetData p C E)) -> HSet)
-  (D : DgnData C E) : DepsReflCohs p 0 :=
+  (C: νSetData p)
+  (E: mkFrame (dgnDepsRestr C) -> HSet)
+  (E': mkFrame (dgnDepsRestr (mkνSetData p C E)) -> HSet)
+  (D: DgnData C E): DepsReflCohs p 0 :=
   dgnDepsReflCohs C E E'
     D.(reflFrames) D.(reflPaintings)
     D.(idReflRestrFrames) D.(idReflRestrPaintings)
     (D.(cohRestrReflFrames) E').
 
 Definition dgnHasReflFromData {p}
-  (C : νSetData p)
-  (E : mkFrame (dgnDepsRestr C) -> HSet)
-  (E' : mkFrame (dgnDepsRestr (mkνSetData p C E)) -> HSet)
-  (D : DgnData C E) : Type :=
+  (C: νSetData p)
+  (E: mkFrame (dgnDepsRestr C) -> HSet)
+  (E': mkFrame (dgnDepsRestr (mkνSetData p C E)) -> HSet)
+  (D: DgnData C E): Type :=
   dgnHasRefl C E E'
     D.(reflFrames) D.(reflPaintings)
     D.(idReflRestrFrames) D.(idReflRestrPaintings)
     (D.(cohRestrReflFrames) E').
 
 Definition dgnDepsReflCohs2FromData {p}
-  (C : νSetData p)
-  (E : mkFrame (dgnDepsRestr C) -> HSet)
-  (E' : mkFrame (dgnDepsRestr (mkνSetData p C E)) -> HSet)
-  (E'' : mkFrame (dgnDepsRestr (mkνSetData p.+1 (mkνSetData p C E) E')) -> HSet)
-  (D : DgnData C E)
-  (L : dgnHasReflFromData C E E' D):
+  (C: νSetData p)
+  (E: mkFrame (dgnDepsRestr C) -> HSet)
+  (E': mkFrame (dgnDepsRestr (mkνSetData p C E)) -> HSet)
+  (E'': mkFrame (dgnDepsRestr (mkνSetData p.+1 (mkνSetData p C E) E')) -> HSet)
+  (D: DgnData C E)
+  (L: dgnHasReflFromData C E E' D):
   DepsReflCohs2 p 0 :=
   {|
     _depsReflCohs := dgnDepsReflCohsFromData C E E' D;
     _extraDepsCohs2 := TopCoh2Dep (depsCohs2 := dgnDepsCohs2 C E E') E'';
-    _extraDepsRefl := TopReflCohDep (deps := dgnDepsReflCohsFromData C E E' D) L;
+    _extraDepsRefl := TopReflCohDep
+      (deps := dgnDepsReflCohsFromData C E E' D) L;
     _cohReflRestrPaintings := D.(cohReflRestrPaintings) E' L;
   |}.
 
 #[local]
-Instance mkDgnData {p} (C : νSetData p)
-  (E : mkFrame (dgnDepsRestr C) -> HSet)
-  (E' : mkFrame (dgnDepsRestr (mkνSetData p C E)) -> HSet)
-  (D : DgnData C E)
-  (L : dgnHasReflFromData C E E' D) :
+Instance mkDgnData {p} (C: νSetData p)
+  (E: mkFrame (dgnDepsRestr C) -> HSet)
+  (E': mkFrame (dgnDepsRestr (mkνSetData p C E)) -> HSet)
+  (D: DgnData C E)
+  (L: dgnHasReflFromData C E E' D):
   DgnData (mkνSetData p C E) E' :=
 {|
-  reflFrames := (mkReflFrames (dgnDepsReflCohsFromData C E E' D) :
+  reflFrames := (mkReflFrames (dgnDepsReflCohsFromData C E E' D):
     mkReflFrameTypes (dgnDepsRestr (mkνSetData p C E)));
   reflPaintings :=
     mkReflPaintings
@@ -872,22 +875,22 @@ Instance mkDgnData {p} (C : νSetData p)
       (TopReflCohDep2 (deps := dgnDepsReflCohs2FromData C E E' E'' D L) L');
 |}.
 
-Class νDgnSet p (C : νSet p) := {
-  dgnPrefix : (mkνSet C).(prefix) -> Type;
-  dgnData (X : (mkνSet C).(prefix)) : dgnPrefix X -> DgnData (C.(data) X.1) X.2;
+Class νDgnSet p (C: νSet p) := {
+  dgnPrefix: (mkνSet C).(prefix) -> Type;
+  dgnData (X: (mkνSet C).(prefix)): dgnPrefix X -> DgnData (C.(data) X.1) X.2;
 }.
 
-Definition mkDgnPrefix p {C : νSet p} {D : νDgnSet p C}
-  (X : (mkνSet (mkνSet C)).(prefix)) : Type :=
-  { L : D.(dgnPrefix) X.1 &T
+Definition mkDgnPrefix p {C: νSet p} {D: νDgnSet p C}
+  (X: (mkνSet (mkνSet C)).(prefix)): Type :=
+  { L: D.(dgnPrefix) X.1 &T
     dgnHasReflFromData (C.(data) X.1.1) X.1.2 X.2 (D.(dgnData) X.1 L) }.
 
 #[local]
-Definition mkνSetData0 : νSetData 0 :=
+Definition mkνSetData0: νSetData 0 :=
   {|
-    frames := (tt : mkFrameTypes 0 0);
-    paintings := (tt : mkPaintingTypes 0 0 (tt : mkFrameTypes 0 0));
-    restrFrames := (tt : mkRestrFrameTypes (tt : mkPaintingTypes 0 0 (tt : mkFrameTypes 0 0)));
+    frames := (tt: mkFrameTypes 0 0);
+    paintings := (tt: mkPaintingTypes 0 0 (tt: mkFrameTypes 0 0));
+    restrFrames := (tt: mkRestrFrameTypes (tt: mkPaintingTypes 0 0 (tt: mkFrameTypes 0 0)));
     restrPaintings := fun _ => tt;
     cohFrames := fun _ => tt;
     cohPaintings := fun _ _ => tt;
@@ -895,10 +898,10 @@ Definition mkνSetData0 : νSetData 0 :=
 
 #[local]
 Definition mkDgnData0
-  (E : mkFrame (dgnDepsRestr mkνSetData0) -> HSet):
+  (E: mkFrame (dgnDepsRestr mkνSetData0) -> HSet):
   DgnData mkνSetData0 E :=
   {|
-    reflFrames := (tt : mkReflFrameTypes (dgnDepsRestr mkνSetData0));
+    reflFrames := (tt: mkReflFrameTypes (dgnDepsRestr mkνSetData0));
     reflPaintings := tt;
     idReflRestrFrames := tt;
     idReflRestrPaintings := tt;
@@ -907,17 +910,17 @@ Definition mkDgnData0
   |}.
 
 #[local]
-Instance mkνDgnSet0 : νDgnSet 0 mkνSet0 :=
+Instance mkνDgnSet0: νDgnSet 0 mkνSet0 :=
   {|
     dgnPrefix := fun _ => unit;
-    dgnData := fun (X : (mkνSet mkνSet0).(prefix)) _ =>
+    dgnData := fun (X: (mkνSet mkνSet0).(prefix)) _ =>
       match X.1 as X0 return DgnData (mkνSet0.(data) X0) X.2 with
       | tt => mkDgnData0 X.2
       end;
   |}.
 
 #[local]
-Instance mkνDgnSetSn {p} (C : νSet p) (D : νDgnSet p C) :
+Instance mkνDgnSetSn {p} (C: νSet p) (D: νDgnSet p C):
   νDgnSet p.+1 (mkνSet C) :=
   {|
     dgnPrefix := fun X => mkDgnPrefix p (C := C) (D := D) X;
@@ -932,18 +935,18 @@ Fixpoint νDgnSetAt n: νDgnSet n (νSetAt n) :=
   end.
 
 CoInductive νDgnSetFrom n
-  (X : (νSetAt n).(prefix))
-  (M : νSetFrom n X)
-  (L : (νDgnSetAt n).(dgnPrefix) (X; this n X M)) : Type := dcons {
-  dgn : dgnHasReflFromData
-          ((νSetAt n).(data) X)
-          (this n X M)
-          (this n.+1 (X; this n X M) (next n X M))
-          ((νDgnSetAt n).(dgnData) (X; this n X M) L);
-  dgnNext : νDgnSetFrom n.+1 (X; this n X M) (next n X M) (L; dgn);
+  (X: (νSetAt n).(prefix))
+  (M: νSetFrom n X)
+  (L: (νDgnSetAt n).(dgnPrefix) (X; this n X M)): Type := dcons {
+  dgn: dgnHasReflFromData
+    ((νSetAt n).(data) X)
+    (this n X M)
+    (this n.+1 (X; this n X M) (next n X M))
+    ((νDgnSetAt n).(dgnData) (X; this n X M) L);
+  dgnNext: νDgnSetFrom n.+1 (X; this n X M) (next n X M) (L; dgn);
 }.
 
-Definition νDgnSets (X : νSets) := νDgnSetFrom 0 tt X tt.
+Definition νDgnSets (X: νSets) := νDgnSetFrom 0 tt X tt.
 
 End νDgnSet.
 
